Bumping to Coq 8.19.0 and adding Simple Mem Spec for Cheriot. Also fixed a bug in the banked memory implementation related to cheriot tag access

Cheriot/BankedMem.v
@@ -1,4 +1,4 @@
-Require Import Kami.AllNotations ProcKami.Cheriot.Lib ProcKami.Cheriot.Types.
+Require Import Kami.AllNotations ProcKami.Cheriot.Lib ProcKami.Cheriot.Types ProcKami.Cheriot.MemSpecIfc.
 
 Section BankedMem.
   Context `{procParams: ProcParams}.
@@ -33,152 +33,138 @@ Section BankedMem.
       rfData := Bool;
       rfInit := RFNonFile _ (Some (ConstBool false)) |}.
 
-  Variable ty: Kind -> Type.
-  Local Open Scope kami_expr.
-  Local Open Scope kami_action.
+  Section ty.
+    Variable ty: Kind -> Type.
+    Local Open Scope kami_expr.
+    Local Open Scope kami_action.
 
-  Section LoadInst.
-    Variable addr: Addr @# ty.
-    
-    Section CommonIdx.
-      Variable idx idxPlus1: Bit (Nat.log2_up NumMemBytes) @# ty.
-      Variable idxLsb: Bit (Nat.log2_up NumBanks) @# ty.
+    Section LoadInst.
+      Variable addr: Addr @# ty.
+      
+      Section CommonIdx.
+        Variable idx idxPlus1: Bit (Nat.log2_up NumMemBytes) @# ty.
+        Variable idxLsb: Bit (Nat.log2_up NumBanks) @# ty.
 
-      Local Fixpoint instReqCallHelp (mbs: list MemBankParams)
-        (exprs: list (Bit 8 @# ty)) (pos: nat) : ActionT ty (Array (length exprs + length mbs) (Bit 8)). refine
-        match mbs return ActionT ty (Array (length exprs + length mbs) (Bit 8)) with
-        | [] => Ret (BuildArray (nth_Fin' exprs (@Nat.add_0_r _)))
-        | m :: ms => ( LET actualIdx <- ITE ($pos < idxLsb) idxPlus1 idx;
-                       LETA ret <- callReadRegFile (Bit 8) (instRqName m) #actualIdx;
-                       (eq_rect _ _ (instReqCallHelp ms
-                                       (exprs ++ [#ret]) (S pos)) _ _))
-        end.
-      abstract (rewrite app_length, <- Nat.add_assoc; reflexivity).
-      Defined.
-    End CommonIdx.
+        Local Fixpoint instReqCallHelp (mbs: list MemBankParams)
+          (exprs: list (Bit 8 @# ty)) (pos: nat) : ActionT ty (Array (length exprs + length mbs) (Bit 8)). refine
+          match mbs return ActionT ty (Array (length exprs + length mbs) (Bit 8)) with
+          | [] => Ret (BuildArray (nth_Fin' exprs (@Nat.add_0_r _)))
+          | m :: ms => ( LET actualIdx <- ITE ($pos < idxLsb) idxPlus1 idx;
+                         LETA ret <- callReadRegFile (Bit 8) (instRqName m) #actualIdx;
+                         (eq_rect _ _ (instReqCallHelp ms
+                                         (exprs ++ [#ret]) (S pos)) _ _))
+          end.
+        abstract (rewrite app_length, <- Nat.add_assoc; reflexivity).
+        Defined.
+      End CommonIdx.
 
-    Definition InstRet := STRUCT_TYPE {
-                              "inst" :: Inst;
-                              "badLower16?" :: Bool;
-                              "error?" :: Bool;
-                              "fault?" :: Bool;
-                              "justFenceI?" :: Bool
-                            }.
-    
-    Definition instReq: ActionT ty InstRet :=
-      ( LET idx <- ZeroExtendTruncLsb (Nat.log2_up NumMemBytes) addr;
-        LET idxPlus1 <- #idx + $1;
-        LET idxLsb <- ZeroExtendTruncLsb (Nat.log2_up NumBanks) addr;
-        LETA bytes <- instReqCallHelp #idx #idxPlus1 #idxLsb memBankInits [] 0;
-        LET shuffledBytes <- ShuffleArray #bytes #idxLsb;
-        Read justFenceI : Bool <- justFenceIReg;
-        Write justFenceIReg : Bool <- $$false;
-        Ret (STRUCT {
-                 "inst" ::= (ZeroExtendTruncLsb InstSz (pack #shuffledBytes));
-                 "badLower16?" ::= Const ty false;
-                 "error?" ::= Const ty false;
-                 "fault?" ::= Const ty false;
-                 "justFenceI?" ::= #justFenceI } : InstRet @# ty)).
-
-    Definition startFenceIRule: ActionT ty Void :=
-      ( Read startFenceI : Bool <- startFenceIReg;
-        WriteIf #startFenceI Then justFenceIReg : Bool <- $$true;
-        Write startFenceIReg : Bool <- $$false;
-        Retv ).
-  End LoadInst.
-
-  Section LoadStore.
-    Variable isStore: Bool @# ty.
-    Variable addr: Addr @# ty.
-    Variable size: MemSize @# ty.
-    Variable isCap: Bool @# ty.
-    Variable data: FullCapWithTag @# ty.
-    Variable signed: Bool @# ty.
-
-    Section CommonIdx.
-      Variable idx idxPlus1: Bit (Nat.log2_up NumMemBytes) @# ty.
-      Variable idxLsb: Bit (Nat.log2_up NumBanks) @# ty.
-      Variable bytes: Array NumBanks (Bit 8) @# ty.
-
-      Local Fixpoint memReqCallHelp (mbs: list MemBankParams) (pos: nat)
-        (exprs: list (Bit 8 @# ty)) : ActionT ty (Array (length exprs + length mbs) (Bit 8)). refine
-        match mbs with
-        | [] => Ret (BuildArray (nth_Fin' exprs (@Nat.add_0_r _)))
-        | m :: ms => ( LET inpPos <- $pos - idxLsb;
-                       LET actualIdx <- ITE (unpack Bool (ZeroExtendTruncMsb 1 #inpPos)) idxPlus1 idx;
-                       LET isWrite <- (ZeroExtend 1 #inpPos) < size;
-                       If isStore
-                       then ( If #isWrite
-                              then callWriteRegFile (storeRqName m) #actualIdx (bytes @[ #inpPos ])
-                              else Retv;
-                              Ret (Const ty Default) )
-                       else callReadRegFile (Bit 8) (loadRqName m) #actualIdx
-                       as ret;
-                       (eq_rect _ _ (memReqCallHelp ms (S pos) (exprs ++ [#ret])) _ _))
-        end.
-      abstract (rewrite app_length, <- Nat.add_assoc; reflexivity).
-      Defined.
-    End CommonIdx.
-
-    Definition DataRet := STRUCT_TYPE {
-                              "data" :: FullCapWithTag;
-                              "lowestByte" :: Bit (Nat.log2_up NumBanks);
-                              "dataError?" :: Bool;
-                              "dataFault?" :: Bool;
-                              "tagError?" :: Bool;
-                              "tagFault?" :: Bool }.
-
-    Definition loadStoreReq: ActionT ty DataRet.
-      refine
+      Definition instReqImpl: ActionT ty InstRet :=
         ( LET idx <- ZeroExtendTruncLsb (Nat.log2_up NumMemBytes) addr;
           LET idxPlus1 <- #idx + $1;
           LET idxLsb <- ZeroExtendTruncLsb (Nat.log2_up NumBanks) addr;
-          LET capVal <- {< (data @% "cap"), (data @% "val") >};
-          LET bytes <- unpack (Array NumBanks (Bit 8)) (castBits _ #capVal);
-          LETA ldBytes <- memReqCallHelp #idx #idxPlus1 #idxLsb #bytes memBankInits 0 [];
-          LET shuffledLdBytes <- ShuffleArray #ldBytes #idxLsb;
-          LET ldSignVal <- (IF signed
-                            then TruncToDynamicSizeArraySigned #shuffledLdBytes size
-                            else TruncToDynamicSizeArrayUnsigned #shuffledLdBytes size);
-          LET ldVal <- unpack FullCap (castBits _ (pack #ldSignVal));
-          LET straddle <- ZeroExtend 1 #idxLsb + size <= $NumBanks;
-          LET tagIdx : Maybe _ <- Valid (ZeroExtendTruncMsb (Nat.log2_up (NumMemBytes/2)) #idx);
-          LET tagIdxPlus1 : Maybe _ <- (STRUCT { "valid" ::= #straddle;
-                                                 "data" ::= ZeroExtendTruncMsb (Nat.log2_up (NumMemBytes/2))
-                                                              #idxPlus1}: Maybe _ @# ty);
-          LET tagIdxLsbIs0 <- unpack Bool (ZeroExtendTruncLsb 1 #idx);
-          LET tag0Idx <- ITE #tagIdxLsbIs0 #tagIdx #tagIdxPlus1;
-          LET tag1Idx <- ITE #tagIdxLsbIs0 #tagIdxPlus1 #tagIdx;
-          (* For stores, if isCap, then tagIdx is valid and tagIdxPlus1 is invalid,
-             so only one of tag0Idx or tag1Idx is valid *)
-          If isStore
-          then ( If (#tag0Idx @% "valid")
-                 then callWriteRegFile (tagWrite ++ "0")%string (#tag0Idx @% "data")
-                        (ITE isCap (data @% "tag") $$false)
-                 else Retv;
-                 If (#tag1Idx @% "valid")
-                 then callWriteRegFile (tagWrite ++ "1")%string (#tag1Idx @% "data")
-                        (ITE isCap (data @% "tag") $$false)
-                 else Retv;
-                 Ret (Const ty Default) )
-          else ( If isCap
-                 then callReadRegFile Bool tagRead #idx
-                 else Ret (Const ty Default)
-                 as retTag;
-                 Ret #retTag )
-          as tag;
+          LETA bytes <- instReqCallHelp #idx #idxPlus1 #idxLsb memBankInits [] 0;
+          LET shuffledBytes <- ShuffleArray #bytes #idxLsb;
+          Read justFenceI : Bool <- justFenceIReg;
+          Write justFenceIReg : Bool <- $$false;
           Ret (STRUCT {
-                   "data" ::= (STRUCT {
-                                   "tag" ::= #tag;
-                                   "cap" ::= #ldVal @% "cap";
-                                   "val" ::= #ldVal @% "val" } : FullCapWithTag @# ty);
-                   "lowestByte" ::= $0;
-                   "dataError?" ::= Const ty false;
-                   "dataFault?" ::= Const ty false;
-                   "tagError?" ::= Const ty false;
-                   "tagFault?" ::= Const ty false } : DataRet @# ty) ).
-      - abstract dischargeDiv8.
-      - abstract (rewrite lengthMemBankInits; dischargeDiv8).
-    Defined.
-  End LoadStore.
+                   "inst" ::= (ZeroExtendTruncLsb InstSz (pack #shuffledBytes));
+                   "badLower16?" ::= Const ty false;
+                   "error?" ::= Const ty false;
+                   "fault?" ::= Const ty false;
+                   "justFenceI?" ::= #justFenceI } : InstRet @# ty)).
+
+    End LoadInst.
+
+    Section LoadStore.
+      Variable isStore: Bool @# ty.
+      Variable addr: Addr @# ty.
+      Variable size: MemSize @# ty.
+      Variable isCap: Bool @# ty.
+      Variable data: FullCapWithTag @# ty.
+      Variable signed: Bool @# ty.
+
+      Section CommonIdx.
+        Variable idx idxPlus1: Bit (Nat.log2_up NumMemBytes) @# ty.
+        Variable idxLsb: Bit (Nat.log2_up NumBanks) @# ty.
+        Variable bytes: Array NumBanks (Bit 8) @# ty.
+
+        Local Fixpoint memReqCallHelp (mbs: list MemBankParams) (pos: nat)
+          (exprs: list (Bit 8 @# ty)) : ActionT ty (Array (length exprs + length mbs) (Bit 8)). refine
+          match mbs with
+          | [] => Ret (BuildArray (nth_Fin' exprs (@Nat.add_0_r _)))
+          | m :: ms => ( LET inpPos <- $pos - idxLsb;
+                         LET actualIdx <- ITE (unpack Bool (ZeroExtendTruncMsb 1 #inpPos)) idxPlus1 idx;
+                         LET isWrite <- (ZeroExtend 1 #inpPos) < size;
+                         If isStore
+                         then ( If #isWrite
+                                then callWriteRegFile (storeRqName m) #actualIdx (bytes @[ #inpPos ])
+                                else Retv;
+                                Ret (Const ty Default) )
+                         else callReadRegFile (Bit 8) (loadRqName m) #actualIdx
+                         as ret;
+                         (eq_rect _ _ (memReqCallHelp ms (S pos) (exprs ++ [#ret])) _ _))
+          end.
+        abstract (rewrite app_length, <- Nat.add_assoc; reflexivity).
+        Defined.
+      End CommonIdx.
+
+      Definition loadStoreReqImpl: ActionT ty DataRet.
+        refine
+          ( LET idx <- ZeroExtendTruncLsb (Nat.log2_up NumMemBytes) addr;
+            LET idxPlus1 <- #idx + $1;
+            LET idxLsb <- ZeroExtendTruncLsb (Nat.log2_up NumBanks) addr;
+            LET capVal <- {< (data @% "cap"), (data @% "val") >};
+            LET bytes <- unpack (Array NumBanks (Bit 8)) (castBits _ #capVal);
+            LETA ldBytes <- memReqCallHelp #idx #idxPlus1 #idxLsb #bytes memBankInits 0 [];
+            LET shuffledLdBytes <- ShuffleArray #ldBytes #idxLsb;
+            LET ldSignVal <- (IF signed
+                              then TruncToDynamicSizeArraySigned #shuffledLdBytes size
+                              else TruncToDynamicSizeArrayUnsigned #shuffledLdBytes size);
+            LET ldVal <- unpack FullCap (castBits _ (pack #ldSignVal));
+            LET straddle <- ZeroExtend 1 #idxLsb + size <= $NumBanks;
+            LET tagIdxBase <- ZeroExtendTruncMsb LgNumTags #idx;
+            LET tagIdxBaseMsb <- ZeroExtendTruncMsb (LgNumTags-1) #tagIdxBase;
+            LET tagIdx : Maybe _ <- Valid #tagIdxBaseMsb;
+            LET tagIdxPlus1 : Maybe _ <- (STRUCT { "valid" ::= #straddle;
+                                                   "data" ::= (#tagIdxBaseMsb + $1)}: Maybe _ @# ty);
+            LET tagIdxLsbIs0 <- unpack Bool (ZeroExtendTruncLsb 1 #tagIdxBase);
+            LET tag0Idx <- ITE #tagIdxLsbIs0 #tagIdx #tagIdxPlus1;
+            LET tag1Idx <- ITE #tagIdxLsbIs0 #tagIdxPlus1 #tagIdx;
+            (* For stores, if isCap, then tagIdx is valid and tagIdxPlus1 is invalid,
+             so only one of tag0Idx or tag1Idx is valid *)
+            If isStore
+            then ( If (#tag0Idx @% "valid")
+                   then callWriteRegFile (tagWrite ++ "0")%string (#tag0Idx @% "data")
+                          (ITE isCap (data @% "tag") $$false)
+                   else Retv;
+                   If (#tag1Idx @% "valid")
+                   then callWriteRegFile (tagWrite ++ "1")%string (#tag1Idx @% "data")
+                          (ITE isCap (data @% "tag") $$false)
+                   else Retv;
+                   Ret (Const ty Default) )
+            else ( If isCap
+                   then callReadRegFile Bool tagRead #idx
+                   else Ret (Const ty Default)
+                   as retTag;
+                   Ret #retTag )
+            as tag;
+            Ret (STRUCT {
+                     "data" ::= (STRUCT {
+                                     "tag" ::= #tag;
+                                     "cap" ::= #ldVal @% "cap";
+                                     "val" ::= #ldVal @% "val" } : FullCapWithTag @# ty);
+                     "lowestByte" ::= $0;
+                     "dataError?" ::= Const ty false;
+                     "dataFault?" ::= Const ty false;
+                     "tagError?" ::= Const ty false;
+                     "tagFault?" ::= Const ty false } : DataRet @# ty) ).
+        - abstract dischargeDiv8.
+        - abstract (rewrite lengthMemBankInits; dischargeDiv8).
+      Defined.
+    End LoadStore.
+  End ty.
+    
+  Instance bankedMem: MemSpecIfc :=
+    {|instReq := instReqImpl;
+      loadStoreReq := loadStoreReqImpl |}.
 End BankedMem.
