Cheriot/MemSpec.v
@@ -1,0 +1,105 @@
+Require Import Kami.AllNotations ProcKami.Cheriot.Lib ProcKami.Cheriot.Types ProcKami.Cheriot.MemSpecIfc.
+
+Section MemSpec.
+  Context `{procParams: ProcParams}.
+  
+  Local Ltac dischargeDiv8 :=
+    unfold NumBanks, FullCap, Cap, CapSz, Data;
+    let H := fresh in
+    destruct (xlenIs32_or_64) as [H | H]; rewrite H; auto.
+  
+  Section ty.
+    Variable ty: Kind -> Type.
+    Local Open Scope kami_expr.
+    Local Open Scope kami_action.
+
+    Section LoadInst.
+      Variable addr: Addr @# ty.
+
+      Section ReadArray.
+        Variable n: nat.
+        Variable arr: Array n (Bit 8) @# ty.
+        Definition readArrayConstSize (size: nat) :=
+          BuildArray (fun (i: Fin.t size) => arr@[addr + $(FinFun.Fin2Restrict.f2n i)]).
+      End ReadArray.
+
+      Definition instReqImpl: ActionT ty InstRet :=
+        ( Read justFenceI : Bool <- justFenceIReg;
+          Write justFenceIReg : Bool <- $$false;
+          Read memArr: Array NumMemBytes (Bit 8) <- memArray;
+          Ret (STRUCT {
+                   "inst" ::= pack (readArrayConstSize #memArr 4);
+                   "badLower16?" ::= Const ty false;
+                   "error?" ::= Const ty false;
+                   "fault?" ::= Const ty false;
+                   "justFenceI?" ::= #justFenceI } : InstRet @# ty)).
+    End LoadInst.
+
+    Section LoadStore.
+      Variable isStore: Bool @# ty.
+      Variable addr: Addr @# ty.
+      Variable size: MemSize @# ty.
+      Variable isCap: Bool @# ty.
+      Variable data: FullCapWithTag @# ty.
+      Variable signed: Bool @# ty.
+
+      Theorem NumBanksNotZero: NumBanks = S (NumBanks - 1).
+      Proof.
+        unfold NumBanks.
+        unfold Xlen, CapSz, Xlen.
+        destruct procParams.
+        destruct xlenIs32_or_64; subst; auto.
+      Qed.
+
+      Definition loadStoreReqImpl: ActionT ty DataRet.
+        refine
+          ( LET idx <- ZeroExtendTruncLsb (Nat.log2_up NumMemBytes) addr;
+            LET idxLsb <- ZeroExtendTruncLsb (Nat.log2_up NumBanks) addr;
+            LET capVal <- {< (data @% "cap"), (data @% "val") >};
+            LET bytes <- unpack (Array NumBanks (Bit 8)) (castBits _ #capVal);
+            Read memArr : Array NumMemBytes (Bit 8) <- memArray;
+            LET ldBytes <- readArrayConstSize addr #memArr NumBanks;
+            LET ldSignVal <- (IF signed
+                              then TruncToDynamicSizeArraySigned #ldBytes size
+                              else TruncToDynamicSizeArrayUnsigned #ldBytes size);
+            LET ldVal <- unpack FullCap (castBits _ (pack #ldSignVal));
+            LET straddle <- ZeroExtend 1 #idxLsb + size <= $NumBanks;
+            LET tagIdx <- ZeroExtendTruncMsb LgNumTags #idx;
+            Read tags: Array NumTags Bool <- tagArray;
+            LET tagVal <- #tags@[#tagIdx];
+            LET updTag <- #tags@[ #tagIdx <- ITE isCap (data @% "tag") $$false];
+            LET updTagPlus1 <- ITE #straddle (#updTag@[ #tagIdx + $1 <- ITE isCap #tagVal $$false]) #updTag;
+            LET stArr <-
+              fold_left (fun newArr i =>
+                           newArr @[addr + $i <-
+                                      ITE ($i < size)
+                                        (match NumBanksNotZero in _ = Y return Array Y (Bit 8) @# ty with
+                                         | eq_refl => #bytes
+                                         end![i]) (#memArr@[addr + $i])])
+                (seq 0 NumBanks) #memArr;
+            If isStore
+            then ( Write memArray: Array NumMemBytes (Bit 8) <- #stArr;
+                   Write tagArray: Array NumTags Bool <- #updTagPlus1;
+                   Ret (Const ty Default) )
+            else ( Ret (ITE isCap #tagVal (Const ty Default)) )
+            as tag;
+            Ret (STRUCT {
+                     "data" ::= (STRUCT {
+                                     "tag" ::= #tag;
+                                     "cap" ::= #ldVal @% "cap";
+                                     "val" ::= #ldVal @% "val" } : FullCapWithTag @# ty);
+                     "lowestByte" ::= $0;
+                     "dataError?" ::= Const ty false;
+                     "dataFault?" ::= Const ty false;
+                     "tagError?" ::= Const ty false;
+                     "tagFault?" ::= Const ty false } : DataRet @# ty) ).
+        - abstract dischargeDiv8.
+        - abstract dischargeDiv8.
+      Defined.
+    End LoadStore.
+  End ty.
+    
+  Instance memSpec: MemSpecIfc :=
+    {|instReq := instReqImpl;
+      loadStoreReq := loadStoreReqImpl |}.
+End MemSpec.
